added STL combinator

examples/low-level/ulib/FStar.SST.fst
@@ -12,19 +12,19 @@ let st_wp (a:Type) = st_wp_h t a
 new_effect STATE = STATE_h t
 effect State (a:Type) (wp:st_wp a) =
        STATE a wp wp
-(* 
-   JK: TODO: change the definitions of the effects so that:
-   - one always have (frame_ids h0 = frame_ids h1)
-   - the topmost frame is always empty (top_frame h0 = Heap.emp)
-*)
-effect STPrime (a:Type) (pre:st_pre) (post: (t -> Tot (st_post a))) =
-       STATE a
-             (fun (p:st_post a) (h:t) -> pre h /\ (forall a h1. post h a h1 ==> p a h1 /\ frame_ids h = frame_ids h1) /\ top_frame h = Heap.emp) (* WP *)
-             (fun (p:st_post a) (h:t) -> forall a h1. (pre h /\ post h a h1) ==> p a h1)          (* WLP *)
+
 effect ST (a:Type) (pre:st_pre) (post: (t -> Tot (st_post a))) =
        STATE a
              (fun (p:st_post a) (h:t) -> pre h /\ (forall a h1. post h a h1 ==> p a h1)) (* WP *)
              (fun (p:st_post a) (h:t) -> (forall a h1. (pre h /\ post h a h1) ==> p a h1))          (* WLP *)
+
+effect STL (a:Type) (pre:st_pre) (post: (t -> Tot (st_post a))) =
+       STATE a
+             (fun (p:st_post a) (h:t) -> pre h /\ (forall a h1. (post h a h1 /\ domain_equality h h1) ==> p a h1)) (* WP *)
+             (fun (p:st_post a) (h:t) -> (forall a h1. (pre h /\ post h a h1 /\ domain_equality h h1) ==> p a h1))          (* WLP *)
+
+effect Stl (a:Type) = STL a (fun h -> True) (fun h0 r h1 -> True)
+
 effect St (a:Type) =
        ST a (fun h -> True) (fun h0 r h1 -> True)
 (* Effect requiring a new frame pushed *)       
@@ -90,16 +90,64 @@ assume val recall_region: i:rid -> ST unit
   (requires (fun m -> True))
   (ensures (fun m0 _ m1 -> m0=m1 /\ contains_frame m1 i))
 
-(* JK: TODO: review and implement *)
-assume val call: #a:Type -> #pre:st_pre -> #post:(t -> Tot (st_post a)) -> (f: unit -> STPrime a pre post) -> 
-  STPrime a
-    (requires (fun h -> (forall h'. fresh_frame h h' ==> pre h')))
-    (ensures (fun h x h' -> (forall h0. (fresh_frame h h0 ==> pre h0) ==> 
-			    (exists h1. post h0 x h1 /\ popped_stack h1 h')) ))
-(* let call #a #pre #post f = push_frame (); let x = f () in pop_frame (); x *)
-
 let lemma_ref_ineq_1 (#a:Type) (#a':Type) (x:ref a) (y:ref a')
   : Lemma (requires (a <> a'))
 	  (ensures (as_ref x =!= as_ref y))
 	  [SMTPat (a <> a')]
   = stack_to_ref_lemma_3 x y
+
+(* Tests *)
+val test_do_nothing: int -> STL int
+  (requires (fun h -> True))
+  (ensures (fun h _ h1 -> True))
+let test_do_nothing x = 
+  push_frame();
+  pop_frame ();
+  x
+
+val test_do_something: s:stacked int -> STL int
+  (requires (fun h -> contains h s))
+  (ensures (fun h r h1 -> contains h s /\ r = sel h s))
+let test_do_something x = 
+  push_frame();
+  let res = !x in
+  pop_frame ();
+  res
+
+val test_do_something_else: s:stacked int -> v:int -> STL unit
+  (requires (fun h -> contains h s))
+  (ensures (fun h r h1 -> contains h1 s /\ v = sel h1 s))
+let test_do_something_else x v = 
+  let h0 = get () in
+  push_frame();
+  let h = get () in
+  x := v;
+  let h' = get () in
+  pop_frame ();
+  let h1 = get () in
+  cut (frame_ids h0 = frame_ids h1);
+  cut (modifies_ref (frameOf x) !{as_ref x} h0 h1); (* Effect incompatibility *)
+  () 
+
+val test_allocate: unit -> Stl unit
+let test_allocate () =
+  push_frame();
+  let h0 = get() in
+  let x = salloc 1 in
+  x := 2;
+  let h1 = get() in
+  cut (modifies_one (top_frame_id h0) h0 h1); (* JK: necessary trigger *)
+  pop_frame ()
+
+val test_nested_stl: unit -> Stl unit
+let test_nested_stl () =
+  let x = test_do_nothing 0 in ()
+
+val test_nested_stl2: unit -> Stl unit
+let test_nested_stl2 () =
+  push_frame ();
+  let h0 = get () in
+  let x = test_do_nothing 0 in 
+  let h1 = get () in
+  cut (modifies_one (top_frame_id h0) h0 h1); (* JK: necessary trigger *)
+  pop_frame ()
