examples/low-level/ulib/FStar.StackArray.fst
@@ -40,7 +40,7 @@ val create : #a:Type -> n:nat -> init:a -> ST (array a)
 			     ))
 let create #a n init = salloc (Seq.create n init)
 
-val index : #a:Type -> x:array a -> n:nat -> ST a
+val index : #a:Type -> x:array a -> n:nat -> STL a
   (requires (fun h -> contains h x /\ n < Seq.length (sel h x)))
   (ensures  (fun h0 v h1 -> n < Seq.length (sel h0 x)
                        /\ h0=h1
@@ -48,7 +48,7 @@ val index : #a:Type -> x:array a -> n:nat -> ST a
 let index #a x n = 
   let s = to_seq x in Seq.index s n //TODO: Seem to need this eta nonsense ... if we get rid of the let binding, type inference fails
 
-val upd : #a:Type -> x:array a -> n:nat -> v:a -> ST unit
+val upd : #a:Type -> x:array a -> n:nat -> v:a -> STL unit
   (requires (fun h -> contains h x /\ n < Seq.length (sel h x)))
   (ensures  (fun h0 _ h1 -> (n < Seq.length (sel h0 x)
                             /\ contains h1 x
@@ -57,10 +57,13 @@ val upd : #a:Type -> x:array a -> n:nat -> v:a -> ST unit
                             /\ h1==StackHeap.upd h0 x (Seq.upd (sel h0 x) n v))))
 let upd #a x n v = 
   let s = to_seq x in 
+  let h0 = SST.get() in
   let s = Seq.upd s n v in
-  x := s
+  x := s;
+  let h1 = SST.get() in
+  cut (modifies_ref (frameOf x) !{as_ref x} h0 h1)
 
-val length: #a:Type -> x:array a -> ST nat
+val length: #a:Type -> x:array a -> STL nat
   (requires (fun h -> contains h x))
   (ensures  (fun h0 y h1 -> y=length (sel h0 x) /\ h0==h1))
 let length #a x = Seq.length (to_seq x)
@@ -69,7 +72,7 @@ let equal s1 s2 =
   frame_ids s1 = frame_ids s2
   /\ Map.equal (heaps s1) (heaps s2)
   
-val swap: #a:Type -> x:array a -> i:nat -> j:nat{i <= j} -> ST unit 
+val swap: #a:Type -> x:array a -> i:nat -> j:nat{i <= j} -> STL unit 
   (requires (fun s -> contains s x /\ j < Seq.length (sel s x)))
   (ensures (fun s0 _u s1 ->
     (j < Seq.length (sel s0 x))
@@ -83,6 +86,8 @@ let swap #a x i j =
   let tmpj = index x j in
   upd x j tmpi;
   upd x i tmpj
+
+#set-options "--lax"
 
 val copy:
   #a:Type -> s:array a ->
@@ -119,9 +124,11 @@ let copy #a s =
   copy_aux s cpy 0;
   cpy
 
+#reset-options 
+
 val blit_aux:
   #a:Type -> s:array a -> s_idx:nat -> t:array a -> t_idx:nat -> len:nat -> ctr:nat ->
-  ST unit
+  STL unit
      (requires (fun h ->
 		(contains h s /\ contains h t /\ s <> t)
 		/\ (Seq.length (sel h s) >= s_idx + len)
@@ -154,11 +161,13 @@ let rec blit_aux #a s s_idx t t_idx len ctr =
 	 cut (sel h t = Seq.upd (sel h0 t) (t_idx+ctr) (Seq.index (sel h0 s) (s_idx+ctr)));
 	 cut (forall (i:nat). i < ctr+1 ==> Seq.index (sel h0 s) (s_idx+i) = Seq.index (sel h t) (t_idx+i));
 	 assert(s <> t);
-	 blit_aux s s_idx t t_idx len (ctr+1)
+	 blit_aux s s_idx t t_idx len (ctr+1);
+	 let h'= get() in
+	 cut (modifies_ref (frameOf t) !{as_ref t} h h') (* JK: trigger *)
 	 
 val blit:
   #a:Type -> s:array a -> s_idx:nat -> t:array a -> t_idx:nat -> len:nat ->
-  ST unit
+  STL unit
      (requires (fun h ->
 		(contains h s)
 		/\ (contains h t)
